theories/TransVal/CombineEnv.v
@@ -62,52 +62,46 @@ Proof.
 Qed.
 
 Lemma renamedApart_contained L E s t Es D
-: Terminates (L, E, s) (L, Es, t)
+: star nc_step (L, E, s) (L, Es, t)
   -> noFun s
   -> renamedApart s D
   -> IL.freeVars t ⊆ fst (getAnn D) ∪ snd (getAnn D).
-
 Proof.
-  intros term_s nf_s ssa_s.
-  general induction term_s; invt noFun; invt renamedApart; try invt F.step; simpl; eauto with cset.
-  - exploit IHterm_s as IH; try reflexivity; eauto.
-    rewrite IH. pe_rewrite. rewrite H9. clear_all; cset_tac.
-  - exploit IHterm_s as IH; try reflexivity; eauto.
-    rewrite IH. pe_rewrite. rewrite <- H8. clear_all; cset_tac.
-  - exploit IHterm_s as IH; try reflexivity; eauto.
-    rewrite IH. pe_rewrite. rewrite <- H8. clear_all; cset_tac.
+  intros Star nf_s ssa_s.
+  general induction Star.
+  - rewrite renamedApart_freeVars; eauto; eauto with cset.
+  - destruct H; simpl in *.
+    invt noFun; invt renamedApart; try invt F.step; simpl;
+      rewrite IHStar; eauto; pe_rewrite.
+    + rewrite H9. clear; cset_tac.
+    + rewrite <- H8. clear; cset_tac.
+    + rewrite <- H8. clear; cset_tac.
+      Grab Existential Variables. eauto. eauto.
 Qed.
 
-Lemma agree_on_ssa_combine:
-  forall D D' L E s t Es Et es et,
-    renamedApart s D
+Lemma nc_step_agree_combine D D' L E s t Es Et es et
+  : renamedApart s D
     -> renamedApart t D'
     -> fst (getAnn D) [=] fst (getAnn D')
     -> disj (snd (getAnn D)) (snd (getAnn D'))
     -> noFun s
     -> noFun t
-    -> Terminates (L, E, s) (L, Es, stmtReturn es)
-    -> Terminates (L, E, t) (L, Et, stmtReturn et)
+    -> star nc_step (L, E, s) (L, Es, stmtReturn es)
+    -> star nc_step (L, E, t) (L, Et, stmtReturn et)
     -> (agree_on eq (Op.freeVars et) Et (combineEnv (fst(getAnn D) ∪ snd(getAnn D)) Es Et)
-        /\ agree_on eq (Op.freeVars es) Es (combineEnv (fst(getAnn D) ∪ snd(getAnn D)) Es Et)).
-
+       /\ agree_on eq (Op.freeVars es) Es (combineEnv (fst(getAnn D) ∪ snd(getAnn D)) Es Et)).
 Proof.
-  intros D D' L E s t Es Et es et.
   intros ssa_s ssa_t agree_fv disj_dv nf_s nf_t sterm tterm.
   split.
-  - edestruct (ssa_move_return D' L E t Et et nf_t ssa_t tterm)
-      as [D'' [ ssaRet [fstSubset sndSubset]]].
-    exploit term_ssa_eval_agree; try eapply sterm; eauto.
-    exploit term_ssa_eval_agree; try eapply tterm; eauto.
+  - exploit nc_step_agree; try eapply sterm; eauto.
+    exploit nc_step_agree; try eapply tterm; eauto.
     exploit (renamedApart_contained L E t (stmtReturn et) Et D') as fv_dv; eauto.
     simpl in *. symmetry.
     eapply agree_on_incl; [ eapply combineEnv_agree_meet | reflexivity ].
     rewrite fv_dv. rewrite <- agree_fv.
     rewrite <- agree_fv in H0. rewrite H in H0; clear H.
     hnf; intros; cset_tac.
-  - edestruct (ssa_move_return D L E s Es es nf_s ssa_s sterm)
-      as [D'' [ssaRet [fstSubset sndSubset]]]; eauto.
-    inv ssaRet. symmetry.
+  - symmetry.
     eapply agree_on_incl; [eapply combineEnv_agree_minus | reflexivity ].
     exploit (renamedApart_contained L E s (stmtReturn es) Es D) as fv_dv; eauto.
     simpl in *.
