theories/TransVal/ComputeProps.v
@@ -1,395 +1,93 @@
-Require Import List CSet.
+Require Import List CSet MapDefined.
 Require Import AutoIndTac Annotation Exp IL RenamedApart Util.
 Require Import SetOperations Sim.
 Require Import SMT NoFun.
 Require Import Guards ILFtoSMT GuardProps.
 
-(** Part 1 of Lemma 1 in the Thesis **)
-Lemma term_ssa_eval_agree L L' s D s' (E:onv val) (E':onv val)
- : renamedApart s D
-   -> noFun s
-   -> Terminates (L, E, s) (L', E', s')
-   -> agree_on eq (fst(getAnn D)) E E'.
+(** All terminating source translations can be modeled with the end environment **)
 
+Lemma terminates_impl_models L s D E s' E'
+  : renamedApart s D
+    -> noFun s
+    -> Terminates (L,E, s) (L, E', s')
+    ->  models (fun (f:pred) (x:list val) => true)  (to_total E')  (translateStmt s source).
 Proof.
-  intros RA NF Trm.
-  general induction Trm; eauto using agree_on_refl.
-  invt renamedApart; try invt F.step;try invt noFun; simpl; eauto.
-  - exploit IHTrm; [ | | reflexivity | reflexivity |]; eauto.
-    pe_rewrite.
-    eapply agree_on_update_inv in H6.
-    eapply agree_on_incl; eauto. cset_tac.
-  - exploit IHTrm; [ | | reflexivity | reflexivity |]; eauto.
-    pe_rewrite. eauto.
-  - exploit IHTrm; [ | | reflexivity | reflexivity |]; eauto.
-    pe_rewrite. eauto.
-Qed.
-
-(** Lemma 13 in Thesis
-Proves that all terminating source translations can be modeled
-with the end environment **)
-Lemma terminates_impl_models :
-forall L s D E s' E',
-renamedApart s D
--> noFun s
--> Terminates (L,E, s) (L, E', s')
-->  models (fun (f:pred) (x:list val) => true)  (to_total E')  (translateStmt s source).
-
-Proof.
-intros L s D E s' E' ren_s noFun_s Term_s.
-general induction Term_s; simpl.
-- assert (X: models (fun (_:pred) (_:list val) => true) (to_total E0) (funcApp (LabI 0) (e::nil))).
-  + simpl; intuition.
-  + eapply models_guardGen_source; simpl. split; eauto.
-      eapply (guard_true_if_eval); eauto.
-- eapply models_guardGen_source; simpl; split; eauto.
-  eapply (guardList_true_if_eval _ E0); eauto.
-- inv H; invt renamedApart; invt noFun; simpl in * |- *; subst; eauto.
-  + eapply models_guardGen_source; simpl; split; eauto.
-    * eapply (guard_true_if_eval _ E'0 e v ); eauto.
-      eapply op_eval_agree; eauto.
-      assert (A: agree_on eq (fst (getAnn (ann1 (D0, D') an))) E0 E'0).
-      { eapply (term_ssa_eval_agree L' L' (stmtLet x (Operation e) s') _ s'0 _ _);
-        econstructor; eauto. }
-      { eapply (agree_on_incl  (bv:=Op.freeVars e) (lv:=fst (getAnn (ann1 (D0, D') an)))); eauto. }
-    * split; eauto; subst.
-      assert (X1: op_eval E'0 (Var x) = Some v).
-      { eapply (op_eval_agree (E:= E0[x <- Some v])) ; eauto.
-        - simpl. eapply (agree_on_incl (bv:={x} ) (lv:= fst (getAnn an))); subst.
-          + eapply (term_ssa_eval_agree L' L' s' _ s'0 _ E'0); eauto.
-          + rewrite H9. unfold fst. cset_tac.
-        - unfold op_eval. unfold update. decide (x===x); eauto; isabsurd. }
-      assert (X2: op_eval E'0 e = Some v).
-      { eapply op_eval_agree; eauto.
-      assert (A: agree_on eq (fst (getAnn (ann1 (D0, D') an))) E0 E'0).
-        - eapply (term_ssa_eval_agree L' L' (stmtLet x (Operation e) s') _ s'0 _ _);
-          econstructor; eauto.
-        - eapply (agree_on_incl  (bv:=Op.freeVars e) (lv:=fst (getAnn (ann1 (D0, D') an)))); eauto. }
-      {  unfold smt_eval;
-        repeat erewrite op_eval_partial_total; eauto.
-      }
-  + assert (X: models  (fun (_:pred) (_:list val) => true) (to_total E'0) ( ite e (translateStmt s' source) (translateStmt b2 source))).
-    * simpl.
-      assert (Op.freeVars e ⊆ fst (getAnn (ann2 (D0, D') ans ant))) by cset_tac.
-      assert (agree_on eq (fst (getAnn (ann2 (D0, D') ans ant))) E' E'0)
-        by ( eapply (term_ssa_eval_agree L' L' (stmtIf e s' b2) _ s'0 _ _); econstructor; eauto).
-      unfold smt_eval.
-      erewrite (op_eval_agree (E:=to_partial (to_total E')) (E':=to_partial (to_total E'0))); eauto.
-      { erewrite op_eval_partial_total; eauto.
+  intros ren_s noFun_s [Term_s Trm].
+  general induction Term_s; simpl.
+  - invt nc_terminal.
+    + eapply models_guardGen_source; simpl. split; eauto.
+      eapply guard_true_if_eval; eauto.
+    + eapply models_guardGen_source; simpl; split; eauto.
+      eapply guardList_true_if_eval; eauto.
+  - exploit nc_step_agree as AGR1; eauto using star_step.
+    destruct H.
+    inv H; invt renamedApart; invt noFun; simpl in * |- *; subst; eauto;
+      exploit nc_step_agree' as AGR2; eauto; simpl in *; pe_rewrite.
+    + eapply models_guardGen_source; simpl; split; [eauto | split; eauto].
+      * eapply (guard_true_if_eval _ E' e v ); eauto.
+        eapply op_eval_agree; eauto.
+        eapply agree_on_incl; eauto.
+      * eapply smt_eval_var; eauto with cset.
+    + erewrite models_guardGen_source. simpl; split.
+      * eapply guard_true_if_eval.
+        eapply op_eval_agree; eauto with cset.
+      * erewrite op_eval_smt_eval; eauto using op_eval_agree with cset.
         rewrite condTrue.
-        eapply IHTerm_s; eauto. }
-      { eapply (agree_on_incl (bv:= Op.freeVars e) (lv:= fst (getAnn (ann2 (D0, D') ans ant)))); eauto.
-        simpl.
-        eapply agree_on_partial; eauto.
-        eapply agree_on_total; eauto. }
-    * erewrite models_guardGen_source.
-      simpl.
-      pose proof (guard_true_if_eval  (fun (_:pred) (_:list val) => true) E'0 e v); eauto.
-      assert (Op.freeVars e ⊆ fst (getAnn (ann2 (D0, D') ans ant))) by cset_tac.
-      assert (agree_on eq (fst (getAnn (ann2 (D0, D') ans ant))) E' E'0)
-        by ( eapply (term_ssa_eval_agree L' L' (stmtIf e s' b2) _ s'0 _ _); econstructor; eauto).
-      assert (op_eval E'0 e = Some v)
-        by (eapply (op_eval_agree (E:=E') (E':=E'0)); eauto;
-        eapply (agree_on_incl (bv:= Op.freeVars e) (lv:= fst (getAnn (ann2 (D0, D') ans ant)))); eauto).
-      split; eauto.
-  + assert (X: models  (fun (_:pred) (_:list val) => true) (to_total E'0) ( ite e (translateStmt b1 source) (translateStmt s' source))).
-    * simpl.
-      assert (Op.freeVars e ⊆ fst (getAnn (ann2 (D0, D') ans ant))) by cset_tac.
-      assert (agree_on eq (fst (getAnn (ann2 (D0, D') ans ant))) E' E'0)
-      by ( eapply (term_ssa_eval_agree L' L' (stmtIf e b1 s') _ s'0 _ _);econstructor;  eauto).
-      unfold smt_eval.
-      erewrite (op_eval_agree (E:=to_partial (to_total E')) (E':=to_partial (to_total E'0))); eauto. simpl.
-      erewrite op_eval_partial_total; eauto.
-      rewrite condFalse.
-      eapply IHTerm_s; eauto.
-      eapply (agree_on_incl (bv:= Op.freeVars e) (lv:= fst (getAnn (ann2 (D0, D') ans ant)))); eauto.
-      eapply agree_on_partial, agree_on_total; eauto.
-    * erewrite models_guardGen_source; simpl.
-      simpl; split; eauto.
-      eapply (guard_true_if_eval  (fun (_:pred) (_:list val) => true) E'0 e v); eauto.
-      assert (Op.freeVars e ⊆ fst (getAnn (ann2 (D0, D') ans ant))) by cset_tac.
-      assert (agree_on eq (fst (getAnn (ann2 (D0, D') ans ant))) E' E'0)
-        by ( eapply (term_ssa_eval_agree L' L' (stmtIf e b1 s') _ s'0 _ _);
-             econstructor; eauto).
-      eapply (op_eval_agree (E:=E') (E':=E'0)); eauto.
-      eapply (agree_on_incl (bv:= Op.freeVars e) (lv:= fst (getAnn (ann2 (D0, D') ans ant)))); eauto.
-Qed.
-
-Lemma terminates_impl_eval L L' E s E' e
-  : noFun s
-    -> Terminates (L, E, s) (L', E',stmtReturn  e)
-    -> exists v, op_eval E' e = Some v.
-Proof.
-  intros NF Trm.
-  general induction Trm; eauto.
-  eapply IHTrm; try reflexivity.
-  inv NF; invt F.step; eauto.
-Qed.
-
-Lemma terminates_impl_evalList L  L' E s E' f el
-  : noFun s
-    -> Terminates (L, E, s) (L', E', stmtApp f el)
-    -> exists v, omap (op_eval E') el = Some v.
-Proof.
-  intros NF Trm.
-  general induction Trm; eauto.
-  eapply IHTrm; try reflexivity.
-  inv NF; invt F.step; eauto.
-Qed.
-
-(** Lemma cannot be proven with star2 step because in the
-goto case, ssa is not proven! **)
-Lemma ssa_move_return:
-  forall D (L:F.labenv) E s E' e,
-    noFun s
-    -> renamedApart s D
-    -> Terminates (L, E, s) (L, E', stmtReturn e)
-    -> exists D', renamedApart (stmtReturn e) D'
-                  /\ fst (getAnn D) ⊆ fst (getAnn D')
-                  /\ snd (getAnn D') ⊆ snd (getAnn D).
-
-Proof.
-  intros. general induction H1; invt renamedApart; invt noFun; try invt F.step.
-  - eexists. split; eauto.
-  - edestruct (IHTerminates an L' (E0[x<-Some v]) s' ); eauto; dcr.
-    pe_rewrite. simpl. eexists; split; eauto.
-    rewrite H7. split; eauto with cset.
-    rewrite <- H13. eauto with cset.
-  - edestruct (IHTerminates ans); eauto; dcr.
-    eexists; split; eauto. simpl.
-    rewrite <- H6. pe_rewrite.
-    rewrite H16, H17. eauto with cset.
-  - edestruct IHTerminates; eauto; dcr.
-    pe_rewrite. simpl.
-    eexists; split; eauto.
-    rewrite <- H6. eauto with cset.
-  - eauto.
-Qed.
-
-(** See Lemma before **)
-Lemma ssa_move_goto:
-  forall D (L:F.labenv) E s E' f el,
-    noFun s
-    -> renamedApart s D
-    -> Terminates (L, E, s) (L, E', stmtApp f el)
-    -> exists D', renamedApart (stmtApp f el) D'
-                  /\ fst (getAnn D) ⊆ fst (getAnn D')
-                  /\ snd (getAnn D') ⊆ snd (getAnn D).
-
-Proof.
-  intros D L E s E' f el nfS ssaS sterm.
-  general induction sterm; invt renamedApart; invt noFun; try invt F.step.
-  - eexists; eauto.
-  - edestruct (IHsterm an L' (E0[x<-Some v]) s' ); eauto; dcr.
-    pe_rewrite. simpl. eexists; split; eauto.
-    rewrite H4. split; eauto with cset.
-    rewrite <- H10. eauto with cset.
-  - edestruct (IHsterm ans); eauto; dcr.
-    eexists; split; eauto. simpl.
-    rewrite <- H3. pe_rewrite.
-    rewrite H13, H14. eauto with cset.
-  - edestruct IHsterm; eauto; dcr.
-    pe_rewrite. simpl.
-    eexists; split; eauto.
-    rewrite <- H3. eauto with cset.
-  - eauto.
+        eauto.
+    + erewrite models_guardGen_source. simpl; split.
+      * eapply guard_true_if_eval.
+        eapply op_eval_agree; eauto with cset.
+      * erewrite op_eval_smt_eval; eauto using op_eval_agree with cset.
+        rewrite condFalse.
+        eauto.
 Qed.
 
 (** Lemmata for Crash **)
 
 Definition failed (s:F.state)  := result (s ) = None.
 
-(** Lemma 3 in the thesis
-Proves that Crashing is independent from the function environment **)
-Lemma crash_swap_fun L1 L2 L1' V V' s s':
-Crash (L1, V, s) (L1', V', s')
--> exists L2', Crash (L2, V, s) (L2', V', s').
-
-Proof.
-  intros crash. general induction crash; eauto using Crash.
-  - eexists. econstructor; eauto.
-    intros [? [? ?]]. eapply H0.
-    invt F.step; try now (do 2 eexists; econstructor; eauto).
-    exfalso. eapply H; eauto.
-  - destruct sigma' as [[L2'' V''] s''].
-    assert (exists L2'', F.step (L2, V, s0) a (L2'', V'', s'')). {
-      inv H; try now (eexists; econstructor; eauto).
-      exfalso; eapply H0; eauto.
-    }
-    destruct H1; eauto. edestruct IHcrash; try reflexivity.
-    eexists; econstructor. eauto. eauto. eauto.
-    Grab Existential Variables. eauto.
-Qed.
-
-(** Part 2 of Lemma 1 in the Thesis *)
-Lemma crash_ssa_eval_agree L L' s D s' (E:onv val) (E':onv val)
-: renamedApart s D
-  ->noFun s
-  -> Crash (L, E, s) (L', E', s')
-  -> agree_on eq (fst (getAnn (D))) E E'.
-
-Proof.
-  intros.
-  general induction H1; invt renamedApart; try invt F.step; try invt noFun; simpl;
-  try reflexivity.
-  - exploit IHCrash; [ | | reflexivity | reflexivity |]; eauto.
-    rewrite H8 in H9; unfold update in H9.
-    simpl in *. hnf; hnf in H9; intros x0 inD0.
-    specialize (H9 x0).
-    assert (x0 ∈ {x; D0}) by cset_tac.
-    specialize (H9 H11); cases in H9; eauto.
-  - exploit IHCrash; [ | | reflexivity | reflexivity |]; eauto.
-    rewrite H9 in H11; eauto.
-  - exploit IHCrash; [ | | reflexivity | reflexivity |]; eauto.
-    rewrite H10 in H11; eauto.
-  - specialize (H0 f Y); isabsurd.
-Qed.
-
-Lemma crash_impl_err:
-  forall (E:onv val) s Es s' L L',
-    noFun s
-    -> Crash (L, E, s) (L', Es, s')
-    -> ( star2 F.step (L,E,s) nil (L', Es, s'))
-       /\ normal2 F.step (L', Es, s') /\ failed (L', Es, s').
-
-Proof.
-  intros E s Es s' L L' nf Crash.
-  general induction Crash.
-  - split; econstructor.
-    +  hnf. intros. destruct H0. destruct H0. inversion H0.
-       rewrite H in def; isabsurd.
-    + unfold failed; eauto.
-   - split; eauto;  econstructor.
-- destruct sigma'. destruct p. inversion nf; subst; try isabsurd.
-  + exploit (IHCrash o s1 Es s' l L') ; try reflexivity; eauto; subst.
-    * inversion H; eauto.
-    * destruct H2; split; eauto.
-      change (star2 F.step (L0, E0, stmtLet x (Operation e) s1) (filter_tau EvtTau nil) (L', Es, s')).
-      econstructor; eauto. destruct a; eauto; isabsurd.
-  + inversion H; exploit (IHCrash o s Es s' l L'); subst; eauto.
-    * split; eauto.
-      change (star2 F.step (l, o, stmtIf e s t) (filter_tau EvtTau nil) (L', Es, s')).
-      econstructor; eauto.
-    * split; eauto.
-      change (star2 F.step (l, o, stmtIf e s1 s) (filter_tau EvtTau nil) (L', Es, s')).
-      econstructor; eauto.
-  + specialize (H0 l0 Y); isabsurd.
-Qed.
-
-Lemma nostep_let:
-  forall L E x e s,
-    normal2 F.step (L, E, stmtLet x (Operation e) s)
-    -> op_eval E e = None.
-
-Proof.
-  intros. case_eq (op_eval E e); intros; eauto.
-  exfalso; apply H. unfold reducible2.
-  exists EvtTau. exists (L, E[x<-Some v],s). econstructor; eauto.
-Qed.
-
-Lemma nostep_if:
-  forall L E e t f,
-    normal2 F.step (L, E, stmtIf e t f)
-    -> op_eval E e = None.
-
-Proof.
-  intros. case_eq (op_eval E e); intros; eauto.
-  exfalso; eapply H; unfold reducible2.
-  exists (EvtTau).
-  case_eq (val2bool v); intros.
-  - exists (L, E, t); econstructor; eauto.
-  - exists (L, E, f); econstructor; eauto.
-Qed.
-
 (** Lemma 11 in the thesis
 Proves that crashing target programs can be modeled by any
 predicate environment and the environment in which they crash **)
-Lemma crash_impl_models:
-  forall L L' D s E Es s',
-    renamedApart s D
-    -> (forall x, x ∈ fst(getAnn D) -> exists v, E x = Some v)
+Lemma crash_impl_models L L' D s E Es s'
+  : renamedApart s D
+    -> defined_on (fst (getAnn D)) E
     -> noFun s
     -> Crash (L, E, s) (L', Es, s')
     -> forall F, models F (to_total Es) (translateStmt s target).
 
 Proof.
-  (** induction over Crash **)
-  intros. general induction H2; simpl.
-  (** C-Goto **)
-  - eapply models_guardGen_target.
-    simpl; intros.
-    pose proof (undefList_models F E0 Y).
-    eapply H5; eauto.
-    intros. eapply H1.
-    inversion H0; simpl; eauto.
-    (** C-Base **)
-  - inversion H4; subst; simpl; eapply models_guardGen_target; simpl; intros; try isabsurd.
-    (** let Statement **)
-    +pose proof (nostep_let L0 E0 x e s H0).
-        pose proof (undef_models F  E0 e).
-        assert (forall x, x ∈ Op.freeVars e -> exists v, E0 x = Some v).
-     * intros; invt renamedApart. specialize (H3 x0). eapply H3.
-       simpl; cset_tac; eauto.
-      (** Contradiction: The expression does not evaluate, but the guard
-       is satisfiable --> undef_models as contradiction **)
-     * specialize(H8 H9 H7 H6); isabsurd.
-       (** conditional **)
-    + pose proof (nostep_if L0 E0 e s t H0).
-      pose proof (undef_models F  E0 e).
-     assert (forall x, x ∈ Op.freeVars e -> exists v, E0 x = Some v).
-     * intros; invt renamedApart. eapply (H3 x). simpl; cset_tac; eauto.
-       (** Same contradiction **)
-     * specialize (H9 H10 H8 H7); isabsurd.
-    + pose proof (undef_models F E0 e).
-         assert (forall x, x ∈ Op.freeVars e -> exists v, E0 x = Some v).
-        { intros; inversion H2; cset_tac. }
-        { eapply H7; eauto. }
-       (** C-Step **)
-  - destruct sigma' as  [[L E'] sc].
+  intros RA DEF NF [Star Crsh] F.
+  general induction Star; simpl.
+  - invt nc_stuck.
+    + eapply models_guardGen_target.
+      simpl; intros.
+      eapply (undefList_models F Es Y); eauto.
+      inv RA; simpl in *. eauto using defined_on_incl.
+    + inv RA; invt noFun; invt notApp; simpl;
+        eapply models_guardGen_target; simpl in *; intros.
+      * exploit nostep_let; eauto.
+        exfalso. eapply undef_models; eauto using defined_on_incl with cset.
+      * exploit nostep_if; eauto.
+        exfalso. eapply undef_models; eauto using defined_on_incl with cset.
+      * eapply undef_models; eauto using defined_on_incl with cset.
+  - exploit nc_step_agree as AGR1; eauto using star_step.
+    destruct H; simpl in *.
     inversion H; intros; subst; try isabsurd;
     invt renamedApart; invt noFun; subst; simpl;
-    eapply models_guardGen_target; simpl; intros.
-    + split.
-     Focus 2.
-     exploit (IHCrash L L' an sc (E0 [x<-Some v]) Es s'); eauto; intros.
-     unfold update. cases; eauto.
-     destruct (H3 x0); eauto; simpl.
-     rewrite H13 in H7; simpl in H7. cset_tac.
-    * assert ( op_eval Es e = Some v /\ op_eval Es (Var x) = Some v).
-    { split.
-      - eapply (op_eval_agree (E:=E0)); eauto.
-        hnf. intros.  hnf in H9. specialize (H9 x0 H7).
-        eapply (crash_ssa_eval_agree L L' (stmtLet x (Operation e) sc) (ann1 (D0, D') an) s' E0 Es);
-          eauto; econstructor; eauto.
-      - eapply (op_eval_agree (E:= E0[x<-Some v])).
-        + hnf. intros; simpl in *.
-          eapply (crash_ssa_eval_agree L L' sc an s' (E0[x<-Some v]) Es); eauto.
-          rewrite H13; simpl. cset_tac.
-        + simpl. unfold update. cases; eauto; isabsurd.
-          }
-    { destruct H7.
-      unfold smt_eval.
-      repeat erewrite op_eval_partial_total; eauto.
-    }
-    +  unfold smt_eval.
-       assert (op_eval Es e = Some v).
-       * eapply (op_eval_agree (E:= E')); eauto.
-         hnf; intros.  hnf in H8.  specialize (H8 x H6).
-         pose proof (crash_ssa_eval_agree L L' (stmtIf e sc b2) (ann2 (D0, D') ans ant) s'  E' Es).
-         eapply H13; eauto; econstructor; eauto.
-       * unfold smt_eval; erewrite op_eval_partial_total; eauto.
-         rewrite condTrue.
-         eapply (IHCrash L L' ans sc E' Es s'); eauto.
-         intros. rewrite H14 in H13. simpl in *; eauto.
-    + unfold smt_eval.
-       assert (op_eval Es e = Some v).
-       * eapply (op_eval_agree (E:= E')); eauto.
-         hnf; intros.  hnf in H8.  specialize (H8 x H6).
-         pose proof (crash_ssa_eval_agree L L' (stmtIf e b1 sc) (ann2 (D0, D') ans ant) s'  E' Es).
-         eapply H13; eauto; econstructor; eauto.
-       * unfold smt_eval; erewrite op_eval_partial_total; eauto.
-         rewrite condFalse.
-         eapply (IHCrash L L' ant sc E' Es s'); eauto.
-         intros. rewrite H15 in H13. simpl in *; eauto.
-    + apply (H0 l Y); auto.
+      eapply models_guardGen_target; simpl in *; intros;
+        exploit nc_step_agree' as AGR2; eauto; simpl in *; pe_rewrite.
+    + split; eauto.
+      * eapply smt_eval_var; eauto with cset.
+      * eapply IHStar; eauto.
+        pe_rewrite. eapply defined_on_update_some.
+        eapply defined_on_incl; eauto. clear; cset_tac.
+    + erewrite op_eval_smt_eval; eauto using op_eval_agree with cset.
+      rewrite condTrue.
+      eapply IHStar; eauto.
+      pe_rewrite. eauto using defined_on_incl with cset.
+    + erewrite op_eval_smt_eval; eauto using op_eval_agree with cset.
+      rewrite condFalse.
+      eapply IHStar; eauto.
+      pe_rewrite. eauto using defined_on_incl with cset.
 Qed.
