theories/TransVal/GuardProps.v
@@ -1,4 +1,4 @@
-Require Import List Arith.
+Require Import List Arith MapDefined.
 Require Import IL Annotation AutoIndTac Exp Fresh Util.
 Require Import SetOperations Sim Var.
 Require Import SMT NoFun.
@@ -42,20 +42,18 @@ Proof.
 Qed.
 
 (** Lemma 8 **)
-Lemma guard_models_impl_eval:
-forall F E e,
-(forall x, x ∈ Op.freeVars e -> exists v,  E x = Some v)
--> models F (to_total E) (undef e)
--> exists v, op_eval E e = Some v.
-
+Lemma guard_models_impl_eval F E e
+  : defined_on (Op.freeVars e) E
+    -> models F (to_total E) (undef e)
+    -> exists v, op_eval E e = Some v.
 Proof.
   intros. general induction e; simpl in *; eauto.
   - destruct (IHe F E); subst; eauto; rewrite H1; simpl.
     eapply unop_eval_total.
   - simpl in *.
     repeat (rewrite models_combine in H0; simpl in H0); intuition; cset_tac.
-    edestruct (IHe1 F); eauto.
-    edestruct (IHe2 F); eauto.
+    edestruct (IHe1 F); eauto using defined_on_incl with cset.
+    edestruct (IHe2 F); eauto using defined_on_incl with cset.
     rewrite H1, H4; simpl.
     cases in H2; simpl in H2.
     + decide (x0 = val_zero).
@@ -65,57 +63,64 @@ Proof.
    + eapply binop_eval_not_div; eauto.
 Qed.
 
+Instance defined_on_morph_incl X `{OrderedType X} Y
+  : Proper (flip Subset ==> eq ==> impl) (@defined_on X _ Y).
+Proof.
+  unfold Proper, respectful, impl; intros; subst.
+  eapply defined_on_incl; eauto.
+Qed.
+
+Instance defined_on_morph_equal X `{OrderedType X} Y
+  : Proper (Equal ==> eq ==> iff) (@defined_on X _ Y).
+Proof.
+  unfold Proper, respectful, flip, impl; intros; subst.
+  eapply eq_incl in H0; dcr; split; intros; eauto using defined_on_incl.
+Qed.
+
 (*  Lemma 8 lifted to lists**)
-Lemma guardlist_impl_eval:
-  forall F E el,
-    (forall x, x ∈ list_union (List.map Op.freeVars el) -> exists v,  E x = Some v)
+Lemma guardlist_impl_eval F E el
+  : defined_on (list_union (List.map Op.freeVars el)) E
     -> models F (to_total E) (undefLift el)
     -> exists v, omap (op_eval E) el = Some v.
 Proof.
   intros.
   general induction el; simpl in *; eauto.
   eapply models_combine in H0; simpl in H0; dcr.
+  rewrite list_union_start_swap in H.
   edestruct IHel; eauto.
-  - eapply op_freeVars_list_agree; eauto.
+  - eauto using defined_on_incl with cset.
   - rewrite H0. edestruct guard_models_impl_eval; eauto.
-    + eapply op_freeVars_list_agree; eauto.
+    + eauto using defined_on_incl with cset.
     + rewrite H3; eexists; simpl; eauto.
 Qed.
 
-(** Lemma 9 in thesis **)
-Lemma guardTrue_if_Terminates_ret:
-  forall L L' E s E' e,
-    noFun s
+Lemma guardTrue_if_Terminates L L' E s E' e
+  : noFun s
     -> Terminates (L, E, s)(L', E', stmtReturn e)
     -> forall F, models F (to_total E') (undef e).
-
 Proof.
-  intros L L' E s E' e noFun_s Terminates_s_ret F.
-  general induction Terminates_s_ret; eauto using guard_true_if_eval.
-  specialize (IHTerminates_s_ret L0 L'0 E' s' E'0 e).
-  inversion H; subst; invt noFun; eauto using IHTerminates_s_ret; eauto.
+  intros noFun_s [Terminates_s_ret Trm] F.
+  general induction Terminates_s_ret; invt nc_terminal.
+  - eauto using guard_true_if_eval.
+  - destruct x' as [[L'' E''] s'']. eauto.
 Qed.
 
-(** Lemma 10 **)
-Lemma guardTrue_if_Terminates_goto:
-forall L L' E s E' f el,
-noFun s
--> Terminates (L, E, s) (L', E' , stmtApp f el)
--> forall F, models F (to_total E') (undefLift el).
-
+Lemma guardTrue_if_Terminates_goto L L' E s E' f el
+  : noFun s
+    -> Terminates (L, E, s) (L', E' , stmtApp f el)
+    -> forall F, models F (to_total E') (undefLift el).
 Proof.
-  intros. general induction H0; eauto using guardList_true_if_eval.
-  specialize (IHTerminates L0 L'0  E' s' E'0 f el).
-  inversion H; subst; invt noFun; eauto using IHTerminates; eauto.
+  intros noFun_s [Terminates_s_ret Trm] F.
+  general induction Terminates_s_ret; invt nc_terminal.
+  - eauto using guardList_true_if_eval.
+  - destruct x' as [[L'' E''] s'']. eauto.
 Qed.
 
 (** Lemma 11 in the Thesis **)
-Lemma undef_models:
-forall F E e,
-(forall x, x ∈ Op.freeVars e -> exists v, E x = Some v)
--> op_eval E e = None
--> ~ models F (to_total E) (undef e).
-
+Lemma undef_models F E e
+  : defined_on (Op.freeVars e) E
+    -> op_eval E e = None
+    -> ~ models F (to_total E) (undef e).
 Proof.
   intros;  hnf;  intros.
   general induction e; simpl in *; try isabsurd.
@@ -126,43 +131,39 @@ Proof.
   - repeat (rewrite models_combine in H1; simpl in H1).
     destruct H1 as [[H1 H2] H3].
     edestruct guard_models_impl_eval; eauto.
-    + eapply op_freeVars_bin_agree; eauto.
+    + eauto using defined_on_incl with cset.
     + edestruct (guard_models_impl_eval F E e1); eauto.
-      * eapply (op_freeVars_bin_agree E e1 e2); eauto.
+      * eauto using defined_on_incl with cset.
       * rewrite H4, H5 in *; simpl in *.
         cases in H3; simpl in H3.
-        eapply H3.
-        unfold smt_eval; erewrite op_eval_partial_total; simpl; eauto.
-        eapply binop_eval_div_zero in H0; subst; eauto.
-        edestruct binop_eval_not_div in H0; eauto.
-        rewrite H6 in H0; congruence.
+        -- eapply H3.
+           unfold smt_eval; erewrite op_eval_partial_total; simpl; eauto.
+           eapply binop_eval_div_zero in H0; subst; eauto.
+        -- edestruct binop_eval_not_div in H0; eauto.
+           rewrite H6 in H0; congruence.
 Qed.
 
-Lemma undefList_models:
-  forall F E el,
-    (forall x, x ∈ list_union (List.map Op.freeVars el) -> exists v, E x = Some v)
+Lemma undefList_models F E el
+  : defined_on (list_union (List.map Op.freeVars el)) E
     -> omap (op_eval E) el = None
     -> ~ models F (to_total E) (undefLift el).
-
 Proof.
   intros.
   general induction el; simpl in *.
   - hnf; intros.
     repeat(rewrite models_combine in H1; simpl in H1).
-    destruct H1.
+    destruct H1. rewrite list_union_start_swap in H.
     pose proof (undef_models F E a).
     monad_inv H0; try isabsurd.
     + eapply H3; eauto.
-      eapply op_freeVars_list_agree; eauto.
+      eauto 20 using defined_on_incl with cset.
     + eapply IHel; eauto.
-      eapply op_freeVars_list_agree; eauto.
+      eauto 20 using defined_on_incl with cset.
 Qed.
 
-Lemma undef_vars_subset:
-  forall e,
-    freeVars (undef e) ⊆ Op.freeVars e.
+Lemma undef_vars_subset e:
+  freeVars (undef e) ⊆ Op.freeVars e.
 Proof.
-  intros e.
   cset_tac.
   induction e; simpl in *; try isabsurd; eauto.
   - rewrite models_combine_vars in H; simpl in H.
