theories/TransVal/TransValSound.v
@@ -23,6 +23,9 @@ Proof.
   rewrite occurVars_freeVars_definedVars. reflexivity.
 Qed.
 
+
+
+
 (** Lemma 12 in the thesis
 Formulas can be extended by a Q that represents the effects of
 the program history
@@ -31,265 +34,92 @@ Lemma unsat_extension L D E E' s s' pol P Q:
 (forall F E, models F (to_total E) Q -> ~ models F (to_total E) (smtAnd (translateStmt s pol) P))
 -> renamedApart s D
 -> noFun s
--> Terminates (L, E, s) (L, E', s')
+-> star nc_step (L, E, s) (L, E', s')
 -> exists Q', (forall F, models F (to_total E')  Q' ) /\
               freeVars Q' ⊆  snd(getAnn D) ∪ fst(getAnn D) /\
               (forall F E, models F (to_total E) (smtAnd Q Q')
                            -> ~ models F (to_total E) (smtAnd (translateStmt s' pol) P)).
 Proof.
-  intros Q_impl_mod ssa_s noFun_s term_s.
-  general induction term_s; destruct pol.
-  - inversion ssa_s.
-    exists smtTrue; simpl; cset_tac.
-  - inversion ssa_s.
-    exists smtTrue; simpl; cset_tac.
-  - inversion ssa_s.
-    exists smtTrue; simpl; cset_tac.
-  - inversion ssa_s.
-    exists smtTrue; simpl; cset_tac.
-  - inv noFun_s.
-    + inv H. inv ssa_s. specialize (IHterm_s L' an (E0 [x <- ⎣ v ⎦]) E'0 s' s'0 source).
-      specialize (IHterm_s P (smtAnd Q (guardGen (undef e) source (constr (Var x) e)))).
-      destruct IHterm_s as [Q' IHterm_s]; inv noFun_s; eauto.
-      * intros F E mod_Q mod_P.
-        specialize (Q_impl_mod F E).
-        simpl in mod_Q.
-        destruct mod_Q as [mod_Q mod_Constr].
-        specialize (Q_impl_mod mod_Q).
-        apply Q_impl_mod; simpl; simpl in mod_P; split; auto.
-        apply models_guardGen_source; apply models_guardGen_source in mod_Constr.
-        simpl in *; destruct mod_Constr, mod_P; split; try split; auto.
-      * exists (smtAnd Q' (guardGen (undef e) source (constr (Var x) e))).
-        destruct IHterm_s as [mod_Q' [fv_subset mod_impl_unsat]].
-        split; try split; eauto.
-        { apply models_guardGen_source; simpl; split.
-          - eapply (guard_true_if_eval _ _ e v); eauto.
-            eapply (op_eval_agree (E:=E0)); eauto. hnf; intros.
-            eapply (term_ssa_eval_agree); eauto; econstructor; eauto.
-          - unfold smt_eval.
-            assert (op_eval E'0 e = Some v).
-            + eapply (op_eval_agree (E:=E0)); eauto; hnf; intros.
-              eapply (term_ssa_eval_agree); eauto; econstructor; eauto.
-            + assert (op_eval E'0 (Var x) = Some v).
-              * eapply (op_eval_agree (E:= E0[x <- Some v])).
-                { hnf. intros. simpl in H4.
-                  eapply (term_ssa_eval_agree L' L' s'); eauto.
-                  rewrite H10; simpl; cset_tac. }
-                { simpl. unfold update. cases; auto. }
-              * rewrite (op_eval_partial_total E'0 (Var x) H4).
-                rewrite (op_eval_partial_total E'0 e H2).
-                eauto.
-        }
-        { rewrite H10 in fv_subset; simpl in *. cset_tac.
-          - hnf in fv_subset. specialize (fv_subset a H4).
-            specialize (H9 a). rewrite H9.
-            cset_tac.
-          - unfold guardGen in H4.
-            cases in H4; simpl in *;
-              rewrite (H9 a); cset_tac.
-            + rewrite undef_vars_subset in H2. cset_tac.
-        }
-        { intros F E mod_Q_Q' mod_trans.
-          apply (mod_impl_unsat F E); auto.
-          - simpl in *.
-            destruct mod_Q_Q' as [mod_Q [mod_E_Q' mod_constr]].
-            split; try split; auto.
-        }
-    + inv H; inv ssa_s.
-      * specialize (IHterm_s L' ans E' E'0 s' s'0 source).
-        specialize (IHterm_s P (smtAnd Q (guardGen (undef e) source (ite e (smtTrue) (smtFalse))))).
-        destruct IHterm_s as [Q' IHterm_s]; inv noFun_s; eauto.
-        { intros F E mod_Q_ite mod_s'.
-          apply (Q_impl_mod F E); simpl in mod_Q_ite, mod_s';
-            destruct mod_Q_ite, mod_s'; simpl;try split; auto.
-          apply models_guardGen_source; simpl; split.
-          - apply models_guardGen_source in H4; simpl in H4; auto.
-          - apply models_guardGen_source in H4; simpl in H4.
-            destruct H4. cases in H16; try auto; isabsurd.
-        }
-        { exists (smtAnd Q' (guardGen (undef e) source (ite e smtTrue smtFalse))).
-          destruct IHterm_s as [mod_Q' [fv_subset mod_impl_unsat]].
-          split; try split; auto.
-          - apply models_guardGen_source; simpl; split.
-            + eapply (guard_true_if_eval _ _ e v); eauto.
-              eapply (op_eval_agree (E:=E')); eauto. hnf; intros.
-              eapply (term_ssa_eval_agree); eauto; econstructor; eauto.
-            + unfold smt_eval.
-              assert (op_eval E'0 e = Some v).
-              * eapply (op_eval_agree (E:=E')); eauto; hnf; intros.
-                eapply (term_ssa_eval_agree); eauto; econstructor; eauto.
-              * rewrite (op_eval_partial_total E'0 e H3).
-                rewrite condTrue; constructor.
-          - simpl. cset_tac.
-            + rewrite <- (H8 a).
-              specialize (fv_subset a H4).
-              rewrite H12 in fv_subset; simpl in fv_subset.
-              cset_tac.
-            + unfold guardGen in H4.
-              rewrite <- (H8 a); cases in H4; cset_tac.
-              simpl in H4. cset_tac.
-              rewrite undef_vars_subset in H3; cset_tac.
-          - intros F E mod_Q_Q' mod_s'.
-            apply (mod_impl_unsat F E).
-            + simpl in *; destruct mod_Q_Q'; auto.
-            + simpl in *; destruct mod_s'; auto.
-        }
-      * specialize (IHterm_s L' ant E' E'0 s' s'0 source).
-        specialize (IHterm_s P (smtAnd Q (guardGen (undef e) source (ite e (smtFalse) (smtTrue))))).
-        destruct IHterm_s as [Q' IHterm_s]; inv noFun_s; eauto.
-        { intros F E mod_Q_ite mod_s'.
-          apply (Q_impl_mod F E); simpl in mod_Q_ite, mod_s';
-            destruct mod_Q_ite, mod_s'; simpl;try split; auto.
-          apply models_guardGen_source; simpl; split.
-          - apply models_guardGen_source in H4; simpl in H4; auto.
-          - apply models_guardGen_source in H4; simpl in H4.
-            destruct H4. cases in H16; try auto; isabsurd.
-        }
-        { exists (smtAnd Q' (guardGen (undef e) source (ite e smtFalse smtTrue))).
-          destruct IHterm_s as [mod_Q' [fv_subset mod_impl_unsat]].
-          split; try split; auto.
-          - apply models_guardGen_source; simpl; split.
-            + eapply (guard_true_if_eval _ _ e v); eauto.
-              eapply (op_eval_agree (E:=E')); eauto. hnf; intros.
-              eapply (term_ssa_eval_agree); eauto; econstructor; eauto.
-            + unfold smt_eval.
-              assert (op_eval E'0 e = Some v).
-              * eapply (op_eval_agree (E:=E')); eauto; hnf; intros.
-                eapply (term_ssa_eval_agree); eauto; econstructor; eauto.
-              * rewrite (op_eval_partial_total E'0 e H3).
-                rewrite condFalse; constructor.
-          - simpl. cset_tac.
-            + rewrite <- (H8 a).
-              specialize (fv_subset a H4).
-              rewrite H13 in fv_subset; simpl in fv_subset.
-              cset_tac.
-            + unfold guardGen in H4.
-              rewrite <- (H8 a); cases in H4; cset_tac.
-              simpl in H4. cset_tac.
-              rewrite undef_vars_subset in H3; cset_tac.
-          - intros F E mod_Q_Q' mod_s'.
-            apply (mod_impl_unsat F E).
-            + simpl in *; destruct mod_Q_Q'; auto.
-            + simpl in *; destruct mod_s'; auto.
-        }
-    + eauto.
-    + isabsurd.
-  - inv noFun_s.
-    + inv H. inv ssa_s. specialize (IHterm_s L' an (E0 [x <- ⎣ v ⎦]) E'0 s' s'0 target).
-      specialize (IHterm_s P (smtAnd Q (guardGen (undef e) target (constr (Var x) e)))).
-      destruct IHterm_s as [Q' IHterm_s]; inv noFun_s; eauto.
-      * intros F E mod_Q mod_P.
-        specialize (Q_impl_mod F E).
-        simpl in mod_Q.
-        destruct mod_Q as [mod_Q mod_Constr].
-        specialize (Q_impl_mod mod_Q).
-        apply Q_impl_mod; simpl; simpl in mod_P; split; auto.
-        apply models_guardGen_target; apply models_guardGen_target in mod_Constr.
-        simpl in *; intros; destruct mod_P; auto.
-      * exists (smtAnd Q' (guardGen (undef e) target (constr (Var x) e))).
-        destruct IHterm_s as [mod_Q' [fv_subset mod_impl_unsat]].
-        split; try split; eauto.
-        { apply models_guardGen_target; simpl; intros.
-          unfold smt_eval.
-          assert (op_eval E'0 e = Some v).
-          - eapply (op_eval_agree (E:=E0)); eauto; hnf; intros.
-            eapply (term_ssa_eval_agree); eauto; econstructor; eauto.
-          - assert (op_eval E'0 (Var x) = Some v).
-            + eapply (op_eval_agree (E:= E0[x <- Some v])).
-              * hnf. intros. simpl in H8.
-                  eapply (term_ssa_eval_agree L' L' s'); eauto.
-                  rewrite H10; simpl; cset_tac.
-              * simpl. unfold update. cases; auto.
-            + rewrite (op_eval_partial_total E'0 (Var x) H8).
-              rewrite (op_eval_partial_total E'0 e H4).
-              eauto.
-        }
-        { rewrite H10 in fv_subset; simpl in *. cset_tac.
-          - hnf in fv_subset. specialize (fv_subset a H4).
-            specialize (H9 a). rewrite H9.
-            cset_tac.
-          - unfold guardGen in H4.
-            cases in H4; simpl in *;
-              rewrite (H9 a); cset_tac.
-            + rewrite undef_vars_subset in H2. cset_tac.
-        }
-        { intros F E mod_Q_Q' mod_trans.
-          apply (mod_impl_unsat F E); auto.
-          - simpl in *.
-            destruct mod_Q_Q' as [mod_Q [mod_E_Q' mod_constr]].
-            split; try split; auto.
-        }
-    + inv H; inv ssa_s.
-      * specialize (IHterm_s L' ans E' E'0 s' s'0 target).
-        specialize (IHterm_s P (smtAnd Q (guardGen (undef e) target (ite e (smtTrue) (smtFalse))))).
-        destruct IHterm_s as [Q' IHterm_s]; inv noFun_s; eauto.
-        { intros F E mod_Q_ite mod_s'.
-          apply (Q_impl_mod F E); simpl in mod_Q_ite, mod_s';
-            destruct mod_Q_ite, mod_s'; simpl;try split; auto.
-          apply models_guardGen_target; simpl.
-          - intros. apply models_guardGen_target in H4. simpl in H4.
-            cases; auto; isabsurd.
-        }
-        { exists (smtAnd Q' (guardGen (undef e) target (ite e smtTrue smtFalse))).
-          destruct IHterm_s as [mod_Q' [fv_subset mod_impl_unsat]].
-          split; try split; auto.
-          - apply models_guardGen_target; simpl.
-            + intros.
-              unfold smt_eval.
-              assert (op_eval E'0 e = Some v).
-              * eapply (op_eval_agree (E:=E')); eauto; hnf; intros.
-                eapply (term_ssa_eval_agree); eauto; econstructor; eauto.
-              * rewrite (op_eval_partial_total E'0 e H4).
-                rewrite condTrue; constructor.
-          - simpl. cset_tac.
-            + rewrite <- (H8 a).
-              specialize (fv_subset a H4).
-              rewrite H12 in fv_subset; simpl in fv_subset.
-              cset_tac.
-            + unfold guardGen in H4.
-              rewrite <- (H8 a); cases in H4; cset_tac.
-              simpl in H4. cset_tac.
-              rewrite undef_vars_subset in H3; cset_tac.
-          - intros F E mod_Q_Q' mod_s'.
-            apply (mod_impl_unsat F E).
-            + simpl in *; destruct mod_Q_Q'; auto.
-            + simpl in *; destruct mod_s'; auto.
-        }
-      * specialize (IHterm_s L' ant E' E'0 s' s'0 target).
-        specialize (IHterm_s P (smtAnd Q (guardGen (undef e) target (ite e (smtFalse) (smtTrue))))).
-        destruct IHterm_s as [Q' IHterm_s]; inv noFun_s; eauto.
-        { intros F E mod_Q_ite mod_s'.
-          apply (Q_impl_mod F E); simpl in mod_Q_ite, mod_s';
-            destruct mod_Q_ite, mod_s'; simpl;try split; auto.
-          apply models_guardGen_target; simpl.
-          - intros. apply models_guardGen_target in H4. simpl in H4; cases; auto; isabsurd.
-        }
-        { exists (smtAnd Q' (guardGen (undef e) target (ite e smtFalse smtTrue))).
-          destruct IHterm_s as [mod_Q' [fv_subset mod_impl_unsat]].
-          split; try split; auto.
-          - apply models_guardGen_target; simpl.
-            + unfold smt_eval.
-              assert (op_eval E'0 e = Some v).
-              * eapply (op_eval_agree (E:=E')); eauto; hnf; intros.
-                eapply (term_ssa_eval_agree); eauto; econstructor; eauto.
-              * rewrite (op_eval_partial_total E'0 e H3).
-                rewrite condFalse; constructor.
-          - simpl. cset_tac.
-            + rewrite <- (H8 a).
-              specialize (fv_subset a H4).
-              rewrite H13 in fv_subset; simpl in fv_subset.
-              cset_tac.
-            + unfold guardGen in H4.
-              rewrite <- (H8 a); cases in H4; cset_tac.
-              simpl in H4. cset_tac.
-              rewrite undef_vars_subset in H3; cset_tac.
-          - intros F E mod_Q_Q' mod_s'.
-            apply (mod_impl_unsat F E).
-            + simpl in *; destruct mod_Q_Q'; auto.
-            + simpl in *; destruct mod_s'; auto.
-        }
-    + eauto.
-    + isabsurd.
+  intros Q_impl_mod RA noFun_s term_s.
+  general induction term_s.
+  - exists smtTrue; simpl; cset_tac.
+  - exploit nc_step_agree as AGR1; eauto using star_step.
+    destruct H; simpl in *.
+    invt noFun; invt renamedApart; invt F.step; invt notApp;
+      exploit nc_step_agree' as AGR2; eauto; simpl in *.
+    + exploit IHterm_s; try reflexivity; eauto.
+      * intros; intro.
+        eapply Q_impl_mod. eauto. simpl.
+        instantiate (1:=(smtAnd P (guardGen (undef e) source (constr (Var x) e))))
+          in H3; simpl in *; dcr.
+        rewrite models_guardGen_source in H12.
+        destruct pol.
+        -- rewrite models_guardGen_source. simpl in *; dcr.
+           repeat (split; eauto).
+        -- rewrite models_guardGen_target. simpl in *; dcr.
+           repeat (split; eauto).
+      * destruct H2 as [P' ?]; simpl in *; dcr.
+        pe_rewrite.
+        eexists (smtAnd P' (guardGen (undef e) source (constr (Var x) e)));
+          repeat split; eauto.
+        -- rewrite models_guardGen_source; simpl; split.
+          ** eapply guard_true_if_eval.
+             eauto using op_eval_agree with cset.
+          ** eapply smt_eval_var; eauto with cset.
+        -- simpl. rewrite freeVars_guardGen, freeVars_undef, !H6; simpl.
+          rewrite H6, H8, H9. pe_rewrite. clear; cset_tac.
+        -- intros; intro. simpl in *.
+           eapply H11; dcr; simpl; eauto.
+    + exploit IHterm_s; try reflexivity; eauto.
+      * intros; intro.
+        eapply Q_impl_mod. eauto. simpl.
+        instantiate (1:=(smtAnd P (guardGen (undef e) source (ite e (smtTrue) (smtFalse))))) in H4; simpl in *; dcr.
+        rewrite models_guardGen_source in H15.
+        destruct pol.
+        -- rewrite models_guardGen_source. simpl in *; dcr.
+           cases in H11; [|isabsurd].
+           repeat (split; eauto).
+        -- rewrite models_guardGen_target. simpl in *; dcr.
+           cases in H11; [|isabsurd].
+           repeat (split; eauto).
+      * destruct H3 as [P' ?]; simpl in *; dcr.
+        pe_rewrite.
+        eexists (smtAnd P' (guardGen (undef e) source (ite e (smtTrue) (smtFalse))));
+          repeat split; eauto.
+        -- rewrite models_guardGen_source; simpl; split.
+          ** eapply guard_true_if_eval.
+             eauto using op_eval_agree with cset.
+          ** erewrite smt_eval_op; eauto with cset.
+             rewrite condTrue; eauto.
+        -- simpl. rewrite freeVars_guardGen, freeVars_undef, !H6; simpl.
+          rewrite H11, <- H8, H6. clear; cset_tac.
+        -- intros; intro. simpl in *.
+           eapply H14; dcr; simpl; eauto.
+    + exploit IHterm_s; try reflexivity; eauto.
+      * intros; intro.
+        eapply Q_impl_mod. eauto. simpl.
+        instantiate (1:=(smtAnd P (guardGen (undef e) source (ite e (smtFalse) (smtTrue))))) in H4; simpl in *; dcr.
+        rewrite models_guardGen_source in H15.
+        destruct pol.
+        -- rewrite models_guardGen_source. simpl in *; dcr.
+           cases in H11; [isabsurd|].
+           repeat (split; eauto).
+        -- rewrite models_guardGen_target. simpl in *; dcr.
+           cases in H11; [isabsurd|].
+           repeat (split; eauto).
+      * destruct H3 as [P' ?]; simpl in *; dcr.
+        pe_rewrite.
+        eexists (smtAnd P' (guardGen (undef e) source (ite e (smtFalse) (smtTrue))));
+          repeat split; eauto.
+        -- rewrite models_guardGen_source; simpl; split.
+          ** eapply guard_true_if_eval.
+             eauto using op_eval_agree with cset.
+          ** erewrite smt_eval_op; eauto with cset.
+             rewrite condFalse; eauto.
+        -- simpl. rewrite freeVars_guardGen, freeVars_undef, !H6; simpl.
+          rewrite H11, <- H8, H6. clear; cset_tac.
+        -- intros; intro. simpl in *.
+           eapply H14; dcr; simpl; eauto.
 Qed.
 
 Lemma predeval_uneq_ret E et es e e' P
@@ -352,7 +182,7 @@ Qed.
 
 (** Case 1 of final theorem.
 Given source program s, target program t, if [s]^+ /\ [t]^- is unsatisfiable
-the two programs must be equivalent **)
+the two programs are equivalent **)
 Lemma tval_term_sound L D D' E Es Et s s' t t'
   : (forall F E, ~ models F E (smtCheck s t))
     (* Both programs have the same free variables *)
@@ -371,7 +201,8 @@ Lemma tval_term_sound L D D' E Es Et s s' t t'
     -> @sim _ statetype_F _ statetype_F Sim (L, E, s) (L, E, t).
 
 Proof.
-  intros Unsat_check Eq_FVars RenApart ssa_s ssa_t nf_s nf_t val_def term_s term_t.
+  intros Unsat_check Eq_FVars RenApart ssa_s ssa_t nf_s nf_t val_def
+         [star_s trm_s] [star_t trm_t].
   unfold smtCheck in Unsat_check.
   pose proof (extend_not_models _ smtTrue Unsat_check) as extend_mod.
   assert (forall (F : pred -> list val -> bool) (E : onv val),
@@ -381,7 +212,7 @@ Proof.
       by (intros F E0 mod_true;specialize (extend_mod F (to_total E0) mod_true); auto).
   pose proof (unsat_extension L D E Es s s' source (translateStmt t target) smtTrue)
     as extend1.
-  specialize (extend1 extend_mod_partial ssa_s nf_s term_s).
+  specialize (extend1 extend_mod_partial ssa_s nf_s star_s).
   destruct extend1 as [Q [mod_Q [fv_Q Unsat_check2]]].
   pose proof (unsat_extension L D' E Et t t' target (translateStmt s' source) (smtAnd smtTrue Q))
     as extend2.
@@ -395,7 +226,7 @@ Proof.
   - specialize (extend2 sat_Q).
     (** Clean up **)
     clear sat_Q Unsat_check Unsat_check2.
-    specialize (extend2 ssa_t nf_t term_t).
+    specialize (extend2 ssa_t nf_t star_t).
     destruct extend2 as [Q' [mod_Q' [fv_Q' Unsat_st]]].
     (** Construct model for assumption: TODO: Make this a lemma**)
     assert (forall F,
@@ -426,8 +257,8 @@ Proof.
         { hnf; intros.
           unfold combineEnv; cases; try eauto.
           cset_tac.
-          - rewrite <- (term_ssa_eval_agree L L s D s' E Es); auto.
-            rewrite <- (term_ssa_eval_agree L L t D' t' E Et); auto.
+          - rewrite <- (@nc_step_agree L L s D s' E Es); auto.
+            rewrite <- (@nc_step_agree L L t D' t' E Et); auto.
           - pose proof (renamedApart_disj ssa_s).
             rewrite <- (Eq_FVars x) in H0;
               exfalso; eauto.
@@ -442,48 +273,29 @@ Proof.
           eapply (agree_on_incl (lv:= fst (getAnn D') ∪ snd(getAnn D')));
             cset_tac; eauto.
           specialize (fv_Q' a H1); cset_tac. }
-    + pose proof (terminates_impl_star2  L E s L Es s' nf_s term_s)
-        as s_star2.
-      pose proof (terminates_impl_star2 L E  t L Et t' nf_t term_t)
-        as t_star2.
-      destruct s_star2 as [s_star2 [ [es ret_s'] | [f [X fcall_s']]]];
-        destruct t_star2 as [t_star2 [ [et ret_t'] | [g [Y fcall_t']]]].
+    + pose proof (nc_star_step star_s) as s_star2.
+      pose proof (nc_star_step star_t) as t_star2.
+
+      inv trm_s; inv trm_t. simpl in *.
     (** s' = e /\ t' = e' --> must be sim **)
-      *  eapply (simTerm Sim
-                (σ1 := (L, E, s)) (σ1' := (L, Es, stmtReturn es))
-                (σ2 := (L, E, t)) (σ2' := (L, Et, stmtReturn et)));
-           subst; try auto.
-         { simpl.
-           assert (exists evs, op_eval Es es = Some evs)
-             as val_es
-               by (apply (terminates_impl_eval L L E s Es es nf_s term_s)).
-           assert (exists evt, op_eval Et et = Some evt)
-          as val_et
-            by (apply (terminates_impl_eval L L E t Et et nf_t term_t)).
-           destruct val_es as [evs evalEs].
-           destruct val_et as [evt evalEt].
-           rewrite evalEs, evalEt.
-           f_equal.
-           remember (smtAnd (smtAnd smtTrue Q) Q') as P.
-           remember (fst (getAnn D) ∪ snd(getAnn D)) as vars_s.
-           remember (combineEnv vars_s Es Et) as C_env.
-           pose proof (predeval_uneq_ret C_env et es evt evs P).
-           symmetry.
-           destruct (agree_on_ssa_combine D D' L E s t Es Et es et); eauto.
-           subst.
-           eapply H; clear H; intros;
-             try erewrite op_eval_agree; eauto. }
-         { unfold normal2.
-           unfold reducible2.
-           hnf; intros.
-           destruct H as [evt [σ step]].
-           inversion step. }
-         { unfold normal2.
-           unfold reducible2.
-           hnf; intros.
-           destruct H as [evt [σ step]]. inversion step. }
+      *  eapply (simTerm Sim);
+           [| eapply s_star2 | eapply t_star2 |stuck2 | stuck2]; simpl.
+         edestruct terminates_impl_eval; eauto. split; eauto.
+         edestruct terminates_impl_eval; try eapply nf_s; eauto.
+         split; eauto.
+         rewrite H, H2.
+         f_equal.
+         remember (smtAnd (smtAnd smtTrue Q) Q') as P.
+         remember (fst (getAnn D) ∪ snd(getAnn D)) as vars_s.
+         remember (combineEnv vars_s Es Et) as C_env.
+         pose proof (predeval_uneq_ret C_env e0 e x x0 P).
+         symmetry.
+         destruct (nc_step_agree_combine D D' L E s t Es Et e e0); eauto.
+         subst; simpl in *; pe_rewrite.
+         eapply H3; eauto;
+           try erewrite op_eval_agree; eauto.
       * subst. simpl in Unsat_st. exfalso.
-        pose (F:= (fun (l:lab) => if (beq_nat (labN l) (labN (labInc g 1)))
+        pose (F:= (fun (l:lab) => if (beq_nat (labN l) (labN (labInc f 1)))
                                then (fun (x:list val) =>  false)
                                else (fun (x:list val) => true))).
         remember (fst (getAnn D) ∪ snd(getAnn D)) as vars_s.
@@ -494,98 +306,87 @@ Proof.
         { erewrite models_guardGen_target.
           erewrite models_guardGen_source.
           simpl; split; intros; try split.
-          - unfold F in H0.
-            rewrite <- (beq_nat_refl (labN(labInc g 1))) in H0; intuition.
+          - unfold F in H2.
+            rewrite <- (beq_nat_refl (labN(labInc f 1))) in H2; intuition.
           - subst.
             rewrite <- combineEnv_models.
-            + eapply (guardTrue_if_Terminates_ret L L _ s); eauto.
+            + eapply (guardTrue_if_Terminates L L _ s); eauto.
+              split; eauto.
             + rewrite freeVars_undef.
-              hnf; intros.
-              exploit (renamedApart_contained); eauto.
-          - unfold F. destruct g; simpl; eauto.
+              rewrite <- (renamedApart_contained); try eapply ssa_s; simpl; eauto.
+              simpl; eauto.
+          - unfold F. destruct f; simpl; eauto.
         }
       * subst.
         simpl in Unsat_st.
         exfalso.
         pose (F:= (fun (l:lab) => if (beq_nat (labN l) (labN (labInc f 1)))
-                                   then (fun (x:list val) =>  true)
-                             else (fun (x:list val) => false))).
+                               then (fun (x:list val) =>  true)
+                               else (fun (x:list val) => false))).
         remember (fst (getAnn D) ∪ snd(getAnn D)) as vars_s.
         remember (combineEnv vars_s Es Et) as E'.
         specialize (Unsat_st F E' ).
         eapply Unsat_st.
-       { eapply (mod_pre). }
-       { erewrite models_guardGen_target.
-         erewrite models_guardGen_source.
-         simpl; split; intros; try split.
-         - unfold F in H0.
-           simpl in H0.
-           unfold labInc in H0.
-           destruct f.
-           simpl in H0; isabsurd.
-         - subst. rewrite <- combineEnv_models.
-             * eapply (guardTrue_if_Terminates_goto L L _ s); eauto.
-             * rewrite freeVars_undefLift.
-               hnf; intros.
-               exploit renamedApart_contained; eauto.
-         - unfold F. rewrite <- (beq_nat_refl (labN (labInc f 1))); constructor.
-       }
+        { eapply (mod_pre). }
+        { erewrite models_guardGen_target.
+          erewrite models_guardGen_source.
+          simpl; split; intros; try split.
+          - unfold F in H0.
+            simpl in H0.
+            unfold labInc in H0.
+            destruct f.
+            simpl in H0; isabsurd.
+          - subst. rewrite <- combineEnv_models.
+            * eapply (guardTrue_if_Terminates_goto L L _ s); eauto.
+              split; eauto.
+            * rewrite freeVars_undefLift.
+              exploit renamedApart_contained; try eapply ssa_s; eauto.
+          - unfold F. rewrite <- (beq_nat_refl (labN (labInc f 1))); constructor.
+        }
       * subst; eapply sim'_sim.
         eapply sim'_expansion_closed; eauto.
         eapply sim_sim'.
-        decide (f = g).
+        decide (f = f0).
         { subst.
-          destruct (get_dec L (counted g)) as [[[bE bZ bs]]|].
-          - pose proof (terminates_impl_evalList L L E s Es g X nf_s term_s).
-            pose proof (terminates_impl_evalList L L E t Et g Y nf_t term_t).
-            destruct H as [es seval]; destruct H0 as [et teval].
+          destruct (get_dec L (counted f0)) as [[[bE bZ bs]]|].
+          - edestruct (@terminates_impl_evalList L L E s Es f0 Y nf_s);
+              [ split; eauto | ].
+            edestruct (@terminates_impl_evalList L L E t Et f0 Y0 nf_t);
+              [ split; eauto | ].
             pose proof (predeval_uneq_goto
                           (combineEnv (fst(getAnn D) ∪ (snd (getAnn D))) Es Et)
-                          g g Y X et es)
+                          f0 f0 Y0 Y x0 x)
               as equal_goto.
             specialize (equal_goto (smtAnd (smtAnd smtTrue Q) Q')).
-(*            oploit term_ssa_eval_agree; eauto.
-            oploit term_ssa_eval_agree; try eapply term_s; eauto.
-            oploit (ssa_move_goto D L E s Es g X) as ssa_goto; eauto; dcr.
-            erewrite <- combineEnv_omap_op_eval in teval.
-            specialize (equal_goto teval).
-            inv H2; simpl in *.*)
-            exploit (combineEnv_omap_exp_eval_left X (fst(getAnn D) ∪ (snd (getAnn D))) Es Et)
+            exploit (combineEnv_omap_exp_eval_left Y (fst(getAnn D) ∪ (snd (getAnn D))) Es Et)
               as val_agree_left.
-            + pose proof (ssa_move_goto D L E s Es g X) as ssa_goto.
-              destruct ssa_goto as [D'' [ssaGoto [fstSubset sndSubset]]]; eauto.
-              inv ssaGoto; simpl in *.
-              hnf; intros.
-              exploit renamedApart_contained as a_in_fst_snd; try eapply term_s; eauto.
-            + exploit (combineEnv_omap_exp_eval_right Y (fst(getAnn D) ∪ (snd (getAnn D))) Es Et)
+            + exploit renamedApart_contained as a_in_fst_snd; try eapply term_s; eauto.
+            + exploit (combineEnv_omap_exp_eval_right Y0 (fst(getAnn D) ∪ (snd (getAnn D))) Es Et)
                 as val_agree_right.
               * (* freeVars ∩ Ds' agree *)
-                edestruct (ssa_move_goto D' L E t Et g Y)
-                  as [D'' [ ssaGoto [ fstSubset sndSubset ]]]; auto.
+                edestruct (@nc_step_renamedApart D' L E t Et)
+                  as [D'' [ ssaGoto [ fstSubset sndSubset ]]]; eauto.
                 inv ssaGoto; simpl in *.
-                exploit (term_ssa_eval_agree L L s D (stmtApp g X) E Es); auto.
-                exploit (term_ssa_eval_agree L L t D'(stmtApp g Y) E Et); auto.
-                rewrite <- Eq_FVars in H0. rewrite H in H0.
+                exploit (@nc_step_agree L L s); eauto.
+                exploit (@nc_step_agree L L t); eauto.
+                rewrite <- Eq_FVars in H4. rewrite H3 in H4.
                 eapply agree_on_incl; eauto.
-                exploit (renamedApart_contained L E t (stmtApp g Y) Et D'); eauto.
+                exploit (renamedApart_contained L E t); eauto.
                 simpl in *.
-                rewrite H2.
+                rewrite H6, Eq_FVars.
                 pose proof (renamedApart_disj ssa_s).
-                rewrite Eq_FVars.
                 cset_tac.
-              * rewrite seval in val_agree_left.
-                rewrite teval in val_agree_right.
-                specialize (equal_goto val_agree_right val_agree_left).
-              (** Make the result values equal **)
-              { rewrite equal_goto in teval; intros;
-                [ | | eapply Unsat_st]; try auto.
-                pose proof (omap_length op val es (op_eval Es) X seval).
-                pose proof (omap_length op val es (op_eval Et) Y teval).
-                decide (length X = length bZ).
-                - one_step.
-                  + simpl. congruence.
-                  + eapply sim_refl.
-                - no_step.  }
+              * exploit equal_goto; eauto; clear equal_goto.
+                rewrite val_agree_right; eauto.
+                rewrite val_agree_left; eauto.
+                subst.
+                exploit omap_length; eauto.
+                exploit omap_length; try eapply H; eauto.
+                decide (length Y = length bZ).
+                -- one_step.
+                   ++ simpl. congruence.
+                   ++ simpl. eapply sim_refl.
+                -- no_step.
           - no_step; eauto. }
         { exfalso.
           pose (F := (fun l => fun (_:list val) => if [labInc f 1 = l] then true else false)).
@@ -595,17 +396,17 @@ Proof.
           - unfold F; simpl.
             erewrite models_guardGen_source; erewrite models_guardGen_target.
             simpl. split; intros; simpl; try split.
-            + cases in H0; eauto.
-              eapply n. destruct f,g. simpl in *; eapply labeq_incr. simpl; eauto.
-            +  pose proof (terminates_impl_evalList L L E s Es f X ).
-               destruct H; eauto.
-               eapply guardList_true_if_eval; eauto.
-               rewrite (combineEnv_omap_exp_eval_left X (fst(getAnn D) ∪ (snd (getAnn D))) Es Et ); eauto.
-               edestruct (ssa_move_goto D L E s Es f X); eauto; dcr.
-               inv H1.
-               subst; simpl in *.
-               hnf; intros.
-               exploit renamedApart_contained; try eapply term_s; eauto.
+            + cases in H2; eauto.
+              eapply n. destruct f,f0. simpl in *; eapply labeq_incr. simpl; eauto.
+            + pose proof (@terminates_impl_evalList L L E s Es f Y); eauto.
+              destruct H; eauto.
+              hnf; split; eauto.
+              eapply guardList_true_if_eval; eauto.
+              rewrite (combineEnv_omap_exp_eval_left Y (fst(getAnn D) ∪ (snd (getAnn D))) Es Et ); eauto.
+              edestruct (@nc_step_renamedApart D L E s Es); eauto; dcr.
+              inv H3.
+              subst; simpl in *.
+              exploit renamedApart_contained; try eapply star_s; eauto.
             + cases; eauto.
         }
 Qed.
@@ -632,9 +433,9 @@ Lemma tval_sound L D D' E s t:
 
 Proof.
   intros Unsat_check Eq_FVars RenApart ssa_s ssa_t nf_s nf_t val_def.
-  pose proof (noFun_impl_term_crash E s nf_s) as term_crash_s.
+  pose proof (@noFun_impl_term_crash E s nf_s) as term_crash_s.
   destruct term_crash_s as [Es [s' term_crash_s]].
-  pose proof (noFun_impl_term_crash E t nf_t) as term_crash_t.
+  pose proof (@noFun_impl_term_crash E t nf_t) as term_crash_t.
   destruct term_crash_t as [Et [t' term_crash_t]].
   specialize (term_crash_s L); specialize (term_crash_t L).
   (** Case Split for Termination of s and t **)
@@ -669,13 +470,13 @@ Proof.
           rewrite renamedApart_freeVars, renamedApart_occurVars; eauto.
           rewrite <- Eq_FVars. symmetry.
           eapply agree_on_incl; [ eapply combineEnv_agree_meet | reflexivity].
-          exploit term_ssa_eval_agree; try eapply term_s; eauto.
-          exploit crash_ssa_eval_agree; try eapply crash_t; eauto.
+          exploit nc_step_agree; try eapply term_s; eauto.
+          exploit nc_step_agree; try eapply crash_t; eauto.
           rewrite <- Eq_FVars in H2. rewrite H1 in H2; clear H1.
-          hnf; intros. cset_tac; eauto.
+          eapply agree_on_incl; eauto.
+          cset_tac; eauto.
         }
   (** s crasht --> always sim *)
-  - pose proof (crash_impl_err E s Es s' L L nf_s crash_s ) as err.
-    destruct err as [star2_s [normal2_s failed_s']].
-    eapply simErr; eauto.
+  - destruct crash_s.
+    eapply simErr; eauto using nc_star_step, nc_stuck_result_none, nc_stuck_terminal.
 Qed.
